week 1

lean/LoVe/LoVe02_ProgramsAndTheorems_ExerciseSheet.lean
@@ -22,8 +22,9 @@ its argument, or 0 if the argument is 0. For example:
     `pred 7 = 6`
     `pred 0 = 0` -/
 
-def pred : ℕ → ℕ :=
-  sorry
+def pred : ℕ → ℕ
+  | 0 => 0
+  | n => n - 1
 
 /- 1.2. Check that your function works as expected. -/
 
@@ -61,7 +62,8 @@ def someEnv : String → ℤ
   | _   => 201
 
 #eval eval someEnv (AExp.var "x")   -- expected: 3
--- invoke `#eval` here
+#eval eval someEnv (AExp.var "y")   -- expected: 17
+#eval eval someEnv (AExp.var "vector")   -- expected: 201
 
 /- 2.2. The following function simplifies arithmetic expressions involving
 addition. It simplifies `0 + e` and `e + 0` to `e`. Complete the definition so
@@ -71,8 +73,10 @@ operators. -/
 def simplify : AExp → AExp
   | AExp.add (AExp.num 0) e₂ => simplify e₂
   | AExp.add e₁ (AExp.num 0) => simplify e₁
-  -- insert the missing cases here
-  -- catch-all cases below
+  | AExp.mul (AExp.num 0) _ => AExp.num 0
+  | AExp.mul _ (AExp.num 0) => AExp.num 0
+  | AExp.sub e₁ (AExp.num 0) => simplify e₁
+  | AExp.div (AExp.num 0) _ => AExp.num 0
   | AExp.num i               => AExp.num i
   | AExp.var x               => AExp.var x
   | AExp.add e₁ e₂           => AExp.add (simplify e₁) (simplify e₂)
@@ -90,8 +94,7 @@ the property that the value of `e` after simplification is the same as the
 value of `e` before. -/
 
 theorem simplify_correct (env : String → ℤ) (e : AExp) :
-  True :=   -- replace `True` by your theorem statement
-  sorry   -- leave `sorry` alone
+  eval env e = eval env (simplify e) := sorry
 
 
 /- ## Question 3 (**optional**): Map
@@ -99,8 +102,9 @@ theorem simplify_correct (env : String → ℤ) (e : AExp) :
 3.1 (**optional**). Define a generic `map` function that applies a function to
 every element in a list. -/
 
-def map {α : Type} {β : Type} (f : α → β) : List α → List β :=
-  sorry
+def map {α : Type} {β : Type} (f : α → β) : List α → List β
+  | List.nil => List.nil
+  | List.cons head tail => List.cons (f head) (map f tail)
 
 #eval map (fun n ↦ n + 10) [1, 2, 3]   -- expected: [11, 12, 13]
 
@@ -114,5 +118,12 @@ Try to give meaningful names to your theorems. Also, make sure to state the
 second property as generally as possible, for arbitrary types. -/
 
 -- enter your theorem statements here
+
+
+theorem map_identity {a:Type} (xs: List a) :
+  xs = (map (fun x ↦ x) xs) := sorry
+
+theorem map_chain {α:Type} {β:Type} {γ:Type} (xs: List α) (f: α → β) (g: β → γ):
+  map (fun x ↦ g (f x)) xs = map g (map f xs) := sorry
 
 end LoVe
